src/tls/Handshake.fst
@@ -322,7 +322,6 @@ let hs_inv (s:hs) (h: HyperHeap.t) =
   /\ Epochs.containsT s.log h                //Nothing deep about these next two, since they can always 
   /\ HyperHeap.contains_ref s.state h                 //be recovered by 'recall'; carrying them in the invariant saves the trouble
 
-
 let iT (s:hs) rw (h:HyperHeap.t) = 
     match rw with
     | Reader -> Epochs.readerT s.log h
@@ -351,7 +350,7 @@ let frame_iT  (s:hs) (rw:rw) (h0:HH.t) (h1:HH.t) (mods:Set.set rid)
 		   /\ iT s rw h0 = iT s rw h1)
   = frame_stateT s rw h0 h1 mods;
     frame_iT_trivial s rw h0 h1
-    
+
 // returns the epoch for reading or writing
 let eT s rw (h:HyperHeap.t { iT s rw h >= 0 }) = Seq.index (logT s h) (iT s rw h)
 
@@ -364,8 +363,8 @@ val i: s:hs -> rw:rw -> ST int
   (ensures (fun h0 i h1 -> h0 = h1 /\ i = iT s rw h1))
 let i (HS #r0 _ _ _ _ (Epochs _ r w) _) rw =
   match rw with
-  | Reader -> !r
-  | Writer -> !w
+  | Reader -> FStar.Monotonic.RRef.m_read r
+  | Writer -> FStar.Monotonic.RRef.m_read w
 // Platform.Error.unexpected "i: not yet implemented" //TODO:Implement
 
 val handshake_state_init: (cfg:TLSInfo.config) -> (r:role) -> (reg:rid) -> ST (handshake_state r)
